compiler/backend/semantics/backendPropsScript.sml
@@ -48,4 +48,61 @@ Theorem FST_pure_co[simp]
   `FST (pure_co co x) = FST x`
   (Cases_on`x` \\ EVAL_TAC);
 
+(* somewhat generic wrappers for defining standard properties about oracles *)
+
+(* identifiers that appear in the initial state and in oracle steps
+   increase monotonically in some sense. *)
+val oracle_monotonic_def = Define`
+  oracle_monotonic (f : 'a -> 'b set) (R : 'b -> 'b -> bool) (S : 'b set)
+    (orac : num -> 'a) =
+    ((!i j x y. i < j /\ x IN f (orac i) /\ y IN f (orac j) ==> R x y)
+        /\ (! i x y. x IN S /\ y IN f (orac i) ==> R x y))`;
+
+val conjs = MATCH_MP quotientTheory.EQ_IMPLIES (SPEC_ALL oracle_monotonic_def)
+  |> UNDISCH_ALL |> CONJUNCTS |> map DISCH_ALL
+
+Theorem oracle_monotonic_step = hd conjs;
+Theorem oracle_monotonic_init = hd (tl conjs);
+
+Theorem oracle_monotonic_subset:
+  ((St' SUBSET St) /\ (!n. f' (co' n) SUBSET f (co n))) ==>
+  oracle_monotonic f R St co ==>
+  oracle_monotonic f' R St' co'
+Proof
+  fs [oracle_monotonic_def, SUBSET_DEF]
+  \\ metis_tac []
+QED
+
+Theorem oracle_monotonic_shift_subset:
+  ((St' SUBSET (IMAGE ((+) (i : num)) St UNION count i)) /\
+    (!n. f' (co' n) SUBSET (IMAGE ((+) i) (f (co n))))) ==>
+  oracle_monotonic f (<) St co ==>
+  oracle_monotonic f' (<) St' co'
+Proof
+  fs [oracle_monotonic_def]
+  \\ rw []
+  \\ fs [SUBSET_DEF]
+  \\ rpt (first_x_assum (fn t => drule t \\ imp_res_tac t))
+  \\ fs []
+QED
+
+(* oracles that carry around state values that can also be constructed by
+   repeatedly applying the incremental compiler *)
+val is_state_oracle_def = Define`
+  is_state_oracle compile_inc_f co init_state =
+    ((FST (FST (co 0)) = init_state) /\ (!n. FST (FST (co (SUC n)))
+        = FST (compile_inc_f (FST (FST (co n))) (SND (co n)))))`;
+
+Theorem is_state_oracle_shift:
+  is_state_oracle compile_inc_f co st =
+  (FST (FST (co 0)) = st /\ is_state_oracle compile_inc_f (shift_seq 1 co)
+        (FST (compile_inc_f st (SND (co 0)))))
+Proof
+  fs [is_state_oracle_def, shift_seq_def]
+  \\ EQ_TAC \\ rw [] \\ fs [sptreeTheory.ADD_1_SUC]
+  \\ full_simp_tac bool_ss [arithmeticTheory.ONE]
+  \\ Cases_on `n`
+  \\ fs []
+QED
+
 val _ = export_theory();
